Start fixing Model

io/model/Instrument.fst
@@ -7,8 +7,6 @@ open Common
 open IO.Sig
 open DM
 open TC.Checkable
-open TC.Monitorable
-open TC.Instrumentable.IIO
 
 let rev_append_rev_append () : Lemma (
   forall (h le1 le2:trace).
@@ -17,32 +15,46 @@ let rev_append_rev_append () : Lemma (
    by (FStar.Tactics.Derived.l_to_r [`List.append_assoc;`List.rev_append])
       = ()
 
-let rec npnode (t:iio 'a) =
+let rec npnode (t:io 'a) =
   match t with
   | Return _ -> True
   | PartialCall _ _ -> False
   | Call cmd arg fnc -> forall r. npnode (fnc r)
   
-type npiio 'a = t:(iio 'a){npnode t}
+type npio 'a = t:(io 'a){npnode t}
+
+let rec from_io_to_npio (tree:io 'a) (p:hist_post #event 'a) h (_:squash (dm_io_theta tree p h)) : npio 'a =
+  match tree with
+  | Return x -> Return x
+  | Call cmd arg fnc -> 
+      let k : (io_sig.res cmd arg) -> npio 'a = fun i -> begin
+        let p' : hist_post 'a = hist_post_shift p [convert_call_to_event cmd arg i] in
+        let h' = apply_changes h [convert_call_to_event cmd arg i] in
+        assert (dm_io_theta (fnc i) p' h');
+        from_io_to_npio (fnc i) p' h' _
+      end in
+      Call cmd arg k
+  | PartialCall pre fnc ->
+      assert pre;
+      from_io_to_npio (fnc ()) p h _
+
+let from_dm_io_to_npio (tree:dm_io 'a (trivial_hist ())) : npio 'a =
+  from_io_to_npio tree (fun _ _ -> True) [] ()
 
 let rec _instrument
-  (tree : npiio 'a)
+  (tree : npio 'a)
   ('p    : monitorable_prop)
   (piprop:squash (forall h cmd arg. 'p cmd arg h ==> io_pre cmd arg h)) :
   IIOpi (maybe 'a) 'p (fun _ -> True) (fun _ _ _ -> True) =
   match tree with
   | Return r -> (Inl r)
-  | Call GetTrace argz fnc ->
-    let h = get_trace () in
-    let z' : npiio 'a = fnc h in
-    _instrument z' 'p piprop
   | Call cmd argz fnc -> begin
     let d : checkable2 (io_pre cmd) = (
       implies_is_checkable2 (io_sig.args cmd) trace ('p cmd) (io_pre cmd) piprop) in
     (** Check if the runtime check failed, and if yes, return the error **)
     match dynamic_cmd cmd d argz with
     | Inl rez ->
-      let z' : npiio 'a = fnc rez in
+      let z' : npio 'a = fnc rez in
       _instrument z' 'p piprop
     | Inr err -> Inr err
   end
