io/model/DM.MIO.fst
@@ -1,74 +1,22 @@
 module DM.MIO
 
 open FStar.Tactics
-open ExtraTactics
 
-open Common
-open DMFree
 open IO.Sig
 open IO.Sig.Call
 open DM.IO
+open Hist
 
-(** MIO models a safe subset of OCaml.
+effect MIO (a:Type) = IOwp a (trivial_hist ())
 
-    Differences between IO and MIO:
-    1) IO is partial (has pre-conditions), MIO is not.
-    2) In IO operations have specification while in MIO they do not have.
-    3) 
+#set-options "--print_implicits"
+let lemma_trivial_wp_theta (cmd:io_cmds) (argz:io_sig.args cmd) :
+  Lemma (trivial_hist #(io_sig.res cmd argz) () `hist_ord #_ #(io_sig.res cmd argz)` dm_io_theta (io_call cmd argz)) = admit ()
 
-Maybe it will be just better to use the old free monad with the IO cmds and no spec?
-**)
-
-let rec np_io (t:io 'a) =
-  match t with
-  | Return _ -> True
-  | PartialCall _ _ -> False
-  | Call cmd arg fnc -> forall r. np_io (fnc r)
-  
-let dm_mio a wp = m:(dm_io a wp){np_io m} 
-
-val dm_mio_return : (a:Type) -> (x:a) -> dm_mio a (hist_return x)
-let dm_mio_return a x = dm_io_return a x
-
-let lemma_io_bind_np_io (#a #b:Type) #w1 #w2 (d1:dm_mio a w1) (d2:(x:a)-> dm_mio b (w2 x)) :
-  Lemma (np_io (dm_io_bind _ _ _ _ d1 d2)) = admit ()  
-
-val dm_mio_bind : 
-      a: Type ->
-      b: Type ->
-      wp_v: hist a ->
-      wp_f: (a -> hist b) ->
-      v: dm_mio a wp_v ->
-      f: (x: a -> dm_mio b (wp_f x))
-    -> dm_mio b (hist_bind wp_v wp_f)
-let dm_mio_bind a b wp_v wp_f v f = 
-  let m:(dm_io b (hist_bind wp_v wp_f)) = dm_io_bind a b wp_v wp_f v f in
-  lemma_io_bind_np_io v f;
-  let m':dm_mio b (hist_bind wp_v wp_f) = m in
-  m'
-
-val dm_mio_subcomp :
-  a: Type -> wp1: Hist.hist a -> wp2: Hist.hist a -> f: dm_mio a wp1
-    -> Pure (dm_mio a wp2) (hist_ord wp2 wp1) (fun _ -> l_True)
-let dm_mio_subcomp a wp1 wp2 f = dm_io_subcomp a wp1 wp2 f
-
-val dm_mio_if_then_else : a:Type u#a -> wp1:hist a -> wp2:hist a -> f:dm_mio a wp1 -> g:dm_mio a wp2 -> bool -> Tot (Type u#(max 1 a))
-let dm_mio_if_then_else a wp1 wp2 f g b = dm_io_if_then_else a wp1 wp2 f g b 
-
-(** No lift from Pure to MIO because MIO is not partial **)
-
-total
-reifiable
-reflectable
-effect {
-  MIOwp (a:Type) (wp : hist a) 
-  with {
-       repr       = dm_mio
-     ; return     = dm_mio_return
-     ; bind       = dm_mio_bind 
-     ; subcomp    = dm_mio_subcomp
-     ; if_then_else = dm_mio_if_then_else
-     }
-}
-
-effect MIO (a:Type) = MIOwp a (fun p h -> forall lt r. p lt r)
+let unsafe_cmd
+  (cmd : io_cmds)
+  (argz : io_sig.args cmd) :
+  MIO (io_sig.res cmd argz) =
+    IOwp?.reflect (
+      lemma_trivial_wp_theta cmd argz;
+      io_call cmd argz)
